compiler/src/examples/lightbulb.v
@@ -35,11 +35,19 @@ Local Existing Instance DefaultRiscvState.
 Local Existing Instance coqutil.Map.SortedListString.map.
 Local Existing Instance coqutil.Map.SortedListString.ok.
 Instance flatToRiscvDef_params: FlatToRiscvDef.FlatToRiscvDef.parameters := {
-  FlatToRiscvDef.FlatToRiscvDef.compile_ext_call argnames fname retnames :=
-    if string_dec fname "nop" then
-      [[Addi Register0 Register0 0]]
-    else
-      nil;
+  FlatToRiscvDef.FlatToRiscvDef.compile_ext_call retnames fname argnames :=
+    if string_dec fname "nop" then [[Addi Register0 Register0 0]]
+    else if string_dec fname "MMIOREAD" then
+           match retnames, argnames with
+           | [res], [addr] => [[ Lw res addr 0 ]]
+           | _, _ => nil
+           end
+    else if string_dec fname "MMIOWRITE" then
+           match retnames, argnames with
+           | [], [addr; val] => [[ Sw addr val 0 ]]
+           | _, _ => nil
+           end
+    else  nil;
   FlatToRiscvDef.FlatToRiscvDef.compile_ext_call_length _ := TODO;
   FlatToRiscvDef.FlatToRiscvDef.compile_ext_call_emits_valid _ _ := TODO;
 }.
@@ -63,11 +71,12 @@ Definition params : Pipeline.parameters. simple refine {|
   Pipeline.src2imp_ops := mapops;
 |}; unshelve (try exact _); apply TODO. Defined.
 Definition flatparams := (FlattenExpr.mk_Syntax_params (@Pipeline.FlattenExpr_parameters params)).
+Definition b : @varname flatparams := "b".
 Instance pipeline_assumptions: @Pipeline.assumptions params. Admitted.
 
 (* stack grows from high addreses to low addresses, first stack word will be written to
    (stack_pastend-4), next stack word to (stack_pastend-8) etc *)
-Definition stack_pastend: Z := 1024.
+Definition stack_pastend: Z := 1024*16.
 Definition compile '(functions, initial, reactive) :=
   compile_prog (p:=params) stack_pastend
      (@Build_Program (FlattenExpr.mk_Semantics_params (@Pipeline.FlattenExpr_parameters params))
@@ -81,10 +90,19 @@ Definition instrencode p : list byte :=
   let word8s := List.flat_map (fun inst => HList.tuple.to_list (LittleEndian.split 4 (encode inst))) p in
   List.map (fun w => Byte.of_Z (word.unsigned w)) word8s.
 
+Require Import coqutil.Z.HexNotation.
 Definition prog := (
-  [iot; lightbulb; recvEthernet; lan9250_readword; spi_write; spi_read],
-  @cmd.skip flatparams,
-  @cmd.call flatparams [] "iot" []).
+  [lan9250_init; lan9250_wait_for_boot; lan9250_mac_write;
+  iot; lightbulb; recvEthernet;  lan9250_writeword; lan9250_readword;
+  spi_xchg; spi_write; spi_read],
+  cmd.seq (@cmd.store flatparams access_size.word (expr.literal (Ox"10012038")) (expr.literal (Z.shiftl (Ox"f") 2))) (
+  cmd.seq (@cmd.store flatparams access_size.word (expr.literal (Ox"10012008")) (expr.literal (Z.shiftl 1 23)))
+  (@cmd.call flatparams ["_"] "lan9250_init" [])),
+  (* @cmd.call flatparams ["_"] "iot" [expr.literal (Ox"80000000")] *)
+  @cmd.call flatparams ["_"] "iot" [expr.literal (1024*4)]
+  (* (@cmd.call flatparams ["a"; "b"] "lan9250_readword" [expr.literal (Ox"64")]) *)
+  (* @cmd.call flatparams ["_"] "spi_write" [expr.literal (Ox"a5")] *)
+).
 
 Import riscv.Utility.InstructionNotations.
 Import bedrock2.Hexdump.
@@ -93,11 +111,14 @@ Set Printing Width 108.
 
 
 Goal True.
-  Time
-  let r := eval vm_compute in (([[
+  pose (let '(functions, initial, reactive) := prog in
+    SortedList.value (snd (functions2Riscv (p:=params) (RegAlloc.map.putmany_of_tuples map.empty functions) (List.map fst functions)))) as symbols.
+  cbv in symbols.
+
+
+  let r := eval cbv in (([[
                          ]] ++ compile prog)%list%Z) in
   pose r as asm.
-  Compute (List.length asm).
   Import bedrock2.NotationsCustomEntry.
 
   (* searching for "addi    x2, x2, -" shows where the functions begin, and the first
